Weidenbach_Book/IsaSAT/IsaSAT_Simplify_Forward_Subsumption_LLVM.thy
@@ -1,7 +1,9 @@
 theory IsaSAT_Simplify_Forward_Subsumption_LLVM
   imports
     IsaSAT_Simplify_Forward_Subsumption
-    IsaSAT_Simplify_Clause_Units_LLVM
+    IsaSAT_Setup_LLVM
+    IsaSAT_Trail_LLVM
+    IsaSAT_Proofs_LLVM
 begin
 
 no_notation WB_More_Refinement.fref (\<open>[_]\<^sub>f _ \<rightarrow> _\<close> [0,60,60] 60)
@@ -57,9 +59,10 @@ sepref_def find_best_subsumption_candidate_code
 lemma isa_push_to_occs_list_st_alt_def:
     \<open>isa_push_to_occs_list_st C S = do {
      L \<leftarrow> find_best_subsumption_candidate C S;
-     let (occs, S) = extract_occs_wl_heur S;
+     let (occs, T) = extract_occs_wl_heur S;
+     ASSERT (length (occs ! nat_of_lit L) < length (get_clauses_wl_heur S));
      occs \<leftarrow> mop_cocc_list_append C occs L;
-     RETURN (update_occs_wl_heur occs S)
+     RETURN (update_occs_wl_heur occs T)
   }\<close>
   by (auto simp: isa_push_to_occs_list_st_def state_extractors
          split: isasat_int_splits)
@@ -73,29 +76,77 @@ sepref_def mop_cocc_list_append_impl
     fold_op_list_list_push_back
   by sepref
 
+lemma empty_tvdom_st_alt_def:
+  \<open>empty_tvdom_st S = do {
+    let (aivdom, S) = extract_vdom_wl_heur S;
+    let aivdom = empty_tvdom aivdom;
+    RETURN (update_vdom_wl_heur aivdom S)
+  }\<close>
+  by (auto simp: isa_push_to_occs_list_st_def state_extractors empty_tvdom_st_def
+         split: isasat_int_splits)
+
+sepref_def empty_tvdom_st_impl
+  is empty_tvdom_st
+  :: \<open>isasat_bounded_assn\<^sup>d \<rightarrow>\<^sub>a isasat_bounded_assn\<close>
+  supply [[goals_limit=1]]
+  unfolding empty_tvdom_st_alt_def
+  by sepref
+
+sepref_register empty_tvdom_st
+
 sepref_def isa_push_to_occs_list_st_impl
   is \<open>uncurry isa_push_to_occs_list_st\<close>
-  :: \<open>sint64_nat_assn\<^sup>k *\<^sub>a isasat_bounded_assn\<^sup>d \<rightarrow>\<^sub>a isasat_bounded_assn\<close>
-  unfolding isa_push_to_occs_list_st_alt_def
-apply sepref_dbg_keep
-apply sepref_dbg_trans_keep
-apply sepref_dbg_trans_step_keep
-apply sepref_dbg_side_unfold
-subgoal premises p
+  :: \<open>[\<lambda>(_, S). isasat_fast_relaxed S]\<^sub>a sint64_nat_assn\<^sup>k *\<^sub>a isasat_bounded_assn\<^sup>d \<rightarrow> isasat_bounded_assn\<close>
+  unfolding isa_push_to_occs_list_st_alt_def isasat_fast_relaxed_def
+  by sepref
+
+sepref_def isa_good_candidate_for_subsumption_impl
+  is \<open>uncurry isa_good_candidate_for_subsumption\<close>
+  :: \<open>isasat_bounded_assn\<^sup>k *\<^sub>a sint64_nat_assn\<^sup>k \<rightarrow>\<^sub>a bool1_assn\<close>
+  unfolding isa_good_candidate_for_subsumption_def
+  by sepref
+
+lemma push_to_tvdom_st_alt_def:
+  \<open>push_to_tvdom_st C S = do {
+    let (av, T) = extract_vdom_wl_heur S;
+    ASSERT (length (get_vdom_aivdom av) \<le> length (get_clauses_wl_heur S));
+    ASSERT (length (get_tvdom_aivdom av) < length (get_clauses_wl_heur S));
+    let av = push_to_tvdom C av;
+    RETURN (update_vdom_wl_heur av T)
+  }\<close>
+  by (auto simp: isa_push_to_occs_list_st_def state_extractors push_to_tvdom_st_def
+         split: isasat_int_splits)
+
+sepref_def push_to_tvdom_st_impl
+  is \<open>uncurry push_to_tvdom_st\<close>
+  :: \<open>[\<lambda>(_, S). isasat_fast_relaxed S]\<^sub>a sint64_nat_assn\<^sup>k *\<^sub>a isasat_bounded_assn\<^sup>d \<rightarrow> isasat_bounded_assn\<close>
+  supply [[goals_limit=1]]
+  unfolding push_to_tvdom_st_alt_def isasat_fast_relaxed_def
+  by sepref
+
+sepref_register isa_good_candidate_for_subsumption sort_cands_by_length
+
+term sort_cands_by_length
+lemma isa_populate_occs_inv_isasat_fast_relaxedI:
+  \<open>isa_populate_occs_inv x cands (a1', a2') \<Longrightarrow> isasat_fast_relaxed x \<Longrightarrow> isasat_fast_relaxed a2'\<close>
+  by (auto simp: isa_populate_occs_inv_def isasat_fast_relaxed_def)
 
 sepref_def isa_populate_occs_code
   is isa_populate_occs
-  :: \<open>isasat_bounded_assn\<^sup>d \<rightarrow>\<^sub>a al_assn' TYPE(64) uint64_nat_assn \<times>\<^sub>a isasat_bounded_assn\<close>
+  :: \<open>[isasat_fast_relaxed]\<^sub>a isasat_bounded_assn\<^sup>d \<rightarrow> isasat_bounded_assn\<close>
   supply [[goals_limit=1]]
   supply [dest] = rdomp_isasat_bounded_assn_length_avdomD
+  supply [intro] = isa_populate_occs_inv_isasat_fast_relaxedI
   unfolding isa_populate_occs_def access_avdom_at_def[symmetric] length_avdom_def[symmetric]
     al_fold_custom_empty[where 'l=64] Let_def[of \<open>get_avdom _\<close>] Let_def[of \<open>get_occs _\<close>]
+    Let_def[of \<open>get_tvdom _\<close>]
   apply (annot_snat_const \<open>TYPE(64)\<close>)
   apply sepref_dbg_keep
   apply sepref_dbg_trans_keep
   apply sepref_dbg_trans_step_keep
   apply sepref_dbg_side_unfold
   subgoal premises p
+apply auto
   oops
 
 thm isa_populate_occs_def
